change the representation of graphs

eulerScript.sml
@@ -1,43 +1,119 @@
 open HolKernel boolLib bossLib listTheory pred_setTheory arithmeticTheory
-     pairTheory
+     pairTheory;
 
-val _ = new_theory "euler"
+new_theory "euler";
 
-(* PAIRS x l z is the set of (oriented) edges used in a path
-   from x to z going by vertices in l *)
-Definition PAIRS_def[simp]:
-  (PAIRS x [] z = {(x,z)}) /\
-  (PAIRS x (y::l) z = (x,y) INSERT PAIRS y l z)
+(* An undirected graph. This definition of graphs does not permit nodes
+   that do not appear in any edge; these seem somewhat pathological so
+   I just kept it simple. *)
+Definition GRAPH_def:
+  GRAPH G <=> (!x y. (x,y) IN G <=> (y,x) IN G) /\ FINITE G
 End
 
-Theorem FINITE_PAIRS:
-  !l x z. FINITE (PAIRS x l z)
+(* A graph with a single edge between x and y *)
+Definition GRAPH1_def:
+  GRAPH1 (x,y) = {(x,y); (y,x)}
+End
+
+Theorem GRAPH_COMPLETE_INDUCTION:
+  !P. (!G. GRAPH G /\ (!E. GRAPH E /\ E PSUBSET G ==> P E) ==> P G) ==>
+      !G. GRAPH G ==> P G
+Proof
+  gen_tac
+  \\ qspec_then `\G. GRAPH G ==> P G`
+                (mp_tac o BETA_RULE) FINITE_COMPLETE_INDUCTION
+  \\ metis_tac[GRAPH_def]
+QED
+
+Definition ADDE_def:
+  ADDE (x,y) G = (x,y) INSERT (y,x) INSERT G
+End
+
+Definition DELE_def:
+  DELE (x,y) G = G DELETE (x,y) DELETE (y,x)
+End
+
+Theorem GRAPH_RWT[simp]:
+  GRAPH {} /\
+  (!x y. GRAPH (GRAPH1 (x,y))) /\
+  (!G. GRAPH G ==> FINITE G) /\
+  (!G e. GRAPH G ==> GRAPH (ADDE e G)) /\
+  (!G e. GRAPH G ==> GRAPH (DELE e G))
+Proof
+  rw[GRAPH_def,GRAPH1_def]
+  THEN1 metis_tac[]
+  THEN Cases_on `e` \\ rw[ADDE_def,DELE_def] \\ metis_tac[]
+QED
+
+Theorem ADDE_DELE:
+  !G x y. GRAPH G /\ (x,y) IN G ==> ADDE (x,y) (DELE (x,y) G) = G
+Proof
+  rw[ADDE_def,DELE_def]
+  \\ Cases_on `(x,y) = (y,x)`
+  THEN1 (rw[] \\ rw[INSERT_DELETE])
+  THEN1 (
+    `(y,x) IN G` by fs[GRAPH_def]
+    \\ qmatch_abbrev_tac `_ INSERT (_ INSERT INNER DELETE _) = _`
+    \\ `(y,x) IN INNER` by rw[Abbr`INNER`,IN_DELETE]
+    \\ rw[Abbr`INNER`,INSERT_DELETE]
+  )
+QED
+
+Theorem DELETE_PSUBSET:
+  !s x. x IN s ==> (s DELETE x) PSUBSET s
+Proof
+  rw[PSUBSET_DEF,DELETE_SUBSET,EXTENSION] \\ metis_tac[]
+QED
+
+Theorem GRAPH_INDUCT:
+  !P. P {} /\ (!G x y. GRAPH G /\ P G ==> P (ADDE (x,y) G)) ==>
+      !G. GRAPH G ==> P G
+Proof
+  ntac 2 strip_tac
+  \\ ho_match_mp_tac GRAPH_COMPLETE_INDUCTION
+  \\ rw[] \\ Cases_on `G = {}`
+  THEN1 rw[]
+  THEN1 (
+    pop_assum (assume_tac o MATCH_MP CHOICE_DEF)
+    \\ Cases_on `CHOICE G`
+    \\ rename [`(x,y)`]
+    \\ `(y,x) IN G` by fs[GRAPH_def]
+    \\ `G = ADDE (x,y) (DELE (x,y) G)` by rw[ADDE_DELE]
+    \\ pop_assum SUBST1_TAC
+    \\ last_x_assum match_mp_tac \\ rw[]
+    \\ first_x_assum match_mp_tac \\ rw[]
+    \\ metis_tac[DELE_def,DELETE_PSUBSET,DELETE_SUBSET,SUBSET_PSUBSET_TRANS]
+  )
+QED
+
+(* The graph formed by all the edges used in a path from x to z going
+   by the vertices of l in sequence *)
+Definition PAIRS_def[simp]:
+  (PAIRS x [] z = GRAPH1 (x,z)) /\
+  (PAIRS x (y::l) z = ADDE (x,y) (PAIRS y l z))
+End
+
+Theorem GRAPH_PAIRS:
+  !l x z. GRAPH (PAIRS x l z)
 Proof Induct \\ rw[]
 QED
 
-(* (x,y) INE G is true when (x,y) is an edge in the undirected
-   graph G *)
-Definition INE_def: INE (x,y) G = ((x,y) IN G \/ (y,x) IN G)
-End
-val _ = Parse.set_fixity "INE" (Parse.Infix(Parse.NONASSOC, 425))
-(* use term_grammar () to print the current grammar *)
-
 (* A circuit is a path that does not go twice by the same
    undirected edge *)
-val (CIRCUIT_rules, CIRCUIT_ind, _) = Hol_reln`
+Inductive CIRCUIT:
   (CIRCUIT x [] z) /\
-  (~((x,y) INE PAIRS y l z) /\ CIRCUIT y l z ==> CIRCUIT x (y::l) z)`
-
-Definition NEIGHB_def: NEIGHB x G = {y | (x,y) INE G}
+  (~((x,y) IN PAIRS y l z) /\ CIRCUIT y l z ==> CIRCUIT x (y::l) z)
 End
 
-Theorem FINITE_NEIGHB:
+Definition NEIGHB_def:
+  NEIGHB x G = {y | (x,y) IN G}
+End
+
+Theorem FINITE_NEIGHB[simp]:
   !x G. FINITE G ==> FINITE (NEIGHB x G)
 Proof
-  `!x G. NEIGHB x G = IMAGE SND (G INTER ({x} CROSS UNIV)) UNION
-                      IMAGE FST (G INTER (UNIV CROSS {x}))` by
-    (rw[NEIGHB_def,INE_def,EXTENSION]
-     \\ metis_tac[PAIR,FST,SND])
+  `!x G. NEIGHB x G = IMAGE SND (G INTER ({x} CROSS UNIV))` by
+    (rw[NEIGHB_def,EXTENSION] \\ metis_tac[FST,SND,PAIR])
   \\ rw[]
 QED
 
@@ -45,41 +121,40 @@ Definition DEG_def:
   DEG x G = CARD (NEIGHB x G) + if (x,x) IN G then 1 else 0
 End
 
-Theorem DEG_SINGLETON:
-  !x y z. DEG x {(y,z)} =
+(* TODO: Maybe inline this inside DEG_ADDE below and drop GRAPH1 *)
+Theorem DEG_GRAPH1:
+  !x y z. DEG x (GRAPH1 (y,z)) =
           if x <> y /\ x <> z then 0 else
           if y = z then 2 else 1
-Proof rw[DEG_def, NEIGHB_def, INE_def] \\ rpt (fs[])
+Proof rw[DEG_def,NEIGHB_def,GRAPH1_def] \\ rpt (fs[])
 QED
 
-Theorem INE_IN:
-  !x E. (x,x) INE E <=> (x,x) IN E
-Proof rw[INE_def]
+Theorem IN_ADDE:
+  !x y u v E. (x,y) IN (ADDE (u,v) E) <=>
+              (x,y) = (u,v) \/ (x,y) = (v,u) \/ (x,y) IN E
+Proof rw[ADDE_def] \\ eq_tac \\ rw[]
 QED
 
-Theorem INE_INSERT:
-  !x y u v E. (x,y) INE ((u,v) INSERT E) <=>
-              (x,y) INE {(u,v)} \/ (x,y) INE E
-Proof rw[INE_def] \\ metis_tac[]
-QED
-
-Theorem DEG_INSERT_ADD:
-  !x y z E. FINITE E /\ ~((y,z) INE E) ==>
-            DEG x ((y,z) INSERT E) = DEG x {(y,z)} + DEG x E
+Theorem DEG_ADDE:
+  !x y z G. GRAPH G /\ ~((y,z) IN G) ==>
+            DEG x (ADDE (y,z) G) = DEG x (GRAPH1 (y,z)) + DEG x G
 Proof
   simp[DEG_def]
   \\ rpt strip_tac
   \\ qmatch_abbrev_tac `CARD S0 + _ = CARD S1 + (CARD S2 + _)`
-  \\ `S0 = S2 UNION S1` by
-       (unabbrev_all_tac \\ rw[NEIGHB_def,Once INE_INSERT,UNION_DEF])
+  \\ let val neighb_goal_tac =
+       unabbrev_all_tac
+       \\ rw[NEIGHB_def,IN_ADDE,GRAPH1_def,EXTENSION]
+       \\ metis_tac[GRAPH_def]
+     in 
+     `S0 = S2 UNION S1` by neighb_goal_tac
   \\ pop_assum (fn eq => rewrite_tac [eq])
-  \\ `FINITE S1` by rw[Abbr`S1`,FINITE_NEIGHB]
-  \\ `FINITE S2` by rw[Abbr`S2`,FINITE_NEIGHB]
-  \\ `CARD (S2 INTER S1) = 0` by
-       (rw[Abbr`S1`,Abbr`S2`,EXTENSION,NEIGHB_def]
-        \\ fs[INE_def] \\ metis_tac[])
+  \\ `FINITE S1` by rw[Abbr`S1`]
+  \\ `FINITE S2` by rw[Abbr`S2`]
+  \\ `CARD (S2 INTER S1) = 0` by neighb_goal_tac
   \\ rw[CARD_UNION_EQN]
-  \\ fs[INE_IN]
+  \\ rpt (fs[GRAPH1_def,IN_ADDE]) (* Hmm, lots seems to be done here... *)
+  end
 QED
 
 Theorem EULER0:
@@ -90,45 +165,45 @@ Theorem EULER0:
     if x = z then EVEN (DEG x G) else ODD (DEG x G) /\ ODD (DEG z G)
 Proof
   ho_match_mp_tac CIRCUIT_ind
-  \\ conj_tac >| [
-    (* empty list *)
-    rw[DEG_SINGLETON],
+  \\ conj_tac
+  (* empty list *)
+  THEN1 rw[DEG_GRAPH1]
+  THEN1 (
     (* non-empty list *)
     qx_genl_tac [`l`,`x`,`y`,`z`]
     \\ strip_tac \\ pop_assum mp_tac
-    \\ qspecl_then [`l`,`y`,`z`] assume_tac FINITE_PAIRS 
-    \\ simp[ODD_EVEN,DEG_INSERT_ADD,EVEN_ADD]
-    \\ rw[] \\ rw[DEG_SINGLETON,DEG_INSERT_ADD,EVEN_ADD] \\ rw[]
-  ]
+    \\ qspecl_then [`l`,`y`,`z`] assume_tac GRAPH_PAIRS 
+    \\ simp[ODD_EVEN,DEG_ADDE,EVEN_ADD]
+    \\ rw[] \\ rw[DEG_ADDE,DEG_GRAPH1,EVEN_ADD] \\ rw[]
+  )
 QED
 
 Definition NODES_def:
-  NODES G = IMAGE FST G UNION IMAGE SND G
+  NODES G = IMAGE FST G
 End
 
-Theorem NODES_INSERT:
-  !G x y. NODES ((x,y) INSERT G) = x INSERT y INSERT NODES G
-Proof
-  rw[NODES_def] \\ metis_tac[INSERT_UNION_EQ,UNION_COMM]
+Theorem NODES_ADDE:
+  !G x y. NODES (ADDE (x,y) G) = x INSERT y INSERT NODES G
+Proof rw[NODES_def,ADDE_def]
 QED
 
-Theorem INE_NODES_INSERT:
-  !G e. e INE G ==> NODES (e INSERT G) = NODES G
+Theorem IN_NODES_ADDE:
+  !G e. GRAPH G /\ e IN G ==> NODES (ADDE e G) = NODES G
 Proof
   Cases_on `e`
-  \\ rw[NODES_INSERT,INE_def]
+  \\ rw[NODES_ADDE]
   \\ `q IN NODES G /\ r IN NODES G` by
-       (rw[NODES_def] \\ metis_tac[FST,SND])
+       (rw[NODES_def] \\ metis_tac[GRAPH_def,FST,SND])
   \\ metis_tac[ABSORPTION]
 QED
 
-Theorem INE_DEG_INSERT:
-  !G e. e INE G ==> !x. DEG x (e INSERT G) = DEG x G
+Theorem IN_DEG_ADDE:
+  !G e. GRAPH G /\ e IN G ==> !x. DEG x (ADDE e G) = DEG x G
 Proof
   rpt strip_tac
-  \\ `!x y. (x,y) INE e INSERT G <=> (x,y) INE G` by
-       (Cases_on `e` \\ fs[INE_def] \\ metis_tac[])
-  \\ rw[DEG_def,NEIGHB_def] \\ fs[INE_def]
+  \\ `!x y. (x,y) IN (ADDE e G) <=> (x,y) IN G` by
+       (Cases_on `e` \\ rw[IN_ADDE] \\ metis_tac[GRAPH_def])
+  \\ rw[DEG_def,NEIGHB_def]
 QED
 
 Theorem SUM_IMAGE_ADD:
@@ -153,44 +228,41 @@ Proof
 QED
 
 Theorem DEG_NON_NODE:
-  !G x. FINITE G ==> x NOTIN NODES G ==> DEG x G = 0
+  !G x. FINITE G /\ x NOTIN NODES G ==> DEG x G = 0
 Proof
   rw[DEG_def]
   THEN1 (
-    `G = (x,x) INSERT G` by metis_tac[ABSORPTION]
+    `G = ADDE (x,x) G` by (simp[ADDE_def] \\ metis_tac[ABSORPTION])
     \\ pop_assum SUBST1_TAC
-    \\ rw[NODES_INSERT]
+    \\ rw[NODES_ADDE]
   )
   THEN1 (
-    rw[FINITE_NEIGHB]
-    \\ rw[NEIGHB_def,EXTENSION]
-    \\ `(x,x') INE G ==> x IN NODES G` by
-         metis_tac[INE_NODES_INSERT,NODES_INSERT,INE_def,IN_INSERT]
-    \\ metis_tac[]
+    rw[NEIGHB_def,EXTENSION]
+    \\ `NODES ((x,x') INSERT G) = x INSERT NODES G` by rw[NODES_def]
+    \\ metis_tac[ABSORPTION]
   )
 QED
 
 Theorem HANDSHAKE:
-  !G. FINITE G ==> EVEN (SIGMA (\x. DEG x G) (NODES G))
+  !G. GRAPH G ==> EVEN (SIGMA (\x. DEG x G) (NODES G))
 Proof
-  ho_match_mp_tac FINITE_INDUCT
+  ho_match_mp_tac GRAPH_INDUCT
   \\ conj_tac
   THEN1 rw[NODES_def,SUM_IMAGE_THM]
   THEN1 (
-    rw[] \\ pop_assum kall_tac
-    \\ Cases_on `e` \\ rename[`(x,y)`]
-    \\ Cases_on `(x,y) INE G`
-    THEN1 simp[INE_NODES_INSERT,INE_DEG_INSERT]
+    rw[]
+    \\ Cases_on `(x,y) IN G`
+    THEN1 simp[IN_NODES_ADDE,IN_DEG_ADDE]
     THEN1 (
-      `FINITE (NODES ((x,y) INSERT G))` by rw[NODES_def]
-      \\ simp[DEG_INSERT_ADD,EVEN_ADD,SUM_IMAGE_ADD]
-      \\ `EVEN (SIGMA (\x. DEG x G) (NODES ((x,y) INSERT G)))` by
-           (fs[NODES_INSERT,SUM_IMAGE_INSERT]
+      `FINITE (NODES (ADDE (x,y) G))` by rw[NODES_def]
+      \\ simp[DEG_ADDE,EVEN_ADD,SUM_IMAGE_ADD]
+      \\ `EVEN (SIGMA (\x. DEG x G) (NODES (ADDE (x,y) G)))` by
+           (fs[NODES_ADDE,ADDE_def,SUM_IMAGE_INSERT]
             \\ rw[] \\ fs[] \\ rw[DEG_NON_NODE])
-      \\ `FINITE (NODES G)` by rw[NODES_def] (* maybe extract as lemma *)
-      \\ rw[NODES_INSERT,SUM_IMAGE_THM,DELETE_INSERT]
+      \\ `FINITE (NODES G)` by rw[NODES_def]
+      \\ rw[NODES_ADDE,SUM_IMAGE_THM,DELETE_INSERT]
       THEN (
-        rw[DEG_SINGLETON,EVEN_ADD]
+        rw[DEG_GRAPH1,EVEN_ADD]
         \\ `!n. n = 0 ==> EVEN n` by rw[]
         \\ pop_assum match_mp_tac
         \\ rw[SUM_IMAGE_ZERO]
@@ -200,41 +272,29 @@ Proof
 QED
 
 Theorem IN_NODES:
-  !G x. x IN NODES G ==> ?y. (x,y) INE G (* really <=> *)
+  !G x. x IN NODES G ==> ?y. (x,y) IN G (* really <=> *)
 Proof
-  rw[NODES_def,INE_def]
-  (* \\ eq_tac \\ rw[] *)
-  \\ metis_tac[PAIR,SND,FST]
+  rw[NODES_def] (* \\ eq_tac \\ rw[] *) \\ metis_tac[PAIR,SND,FST]
 QED
 
-Theorem DELETE_PSUBSET:
-  !s x. x IN s ==> (s DELETE x) PSUBSET s
-Proof
-  rw[PSUBSET_DEF,DELETE_SUBSET,EXTENSION] \\ metis_tac[]
-QED
+Definition CIRCUIT_OF_def:
+  CIRCUIT_OF G x l z = (CIRCUIT x l z /\ G = PAIRS x l z)
+End
 
-Theorem CIRCUIT_OF_INSERT:
-  !G x y z. ~((x,y) INE G) /\ (?l. CIRCUIT_OF G y l z) ==>
-            ?l. CIRCUIT_OF ((x,y) INSERT G) x l z
+Theorem CIRCUIT_OF_ADDE:
+  !G x y z. (x,y) NOTIN G /\ (?l. CIRCUIT_OF G y l z) ==>
+            ?l. CIRCUIT_OF (ADDE (x,y) G) x l z
 Proof
   rw[CIRCUIT_OF_def]
   \\ qexists_tac `y::l`
   \\ conj_tac
   THEN1 (match_mp_tac (CONJUNCT2 CIRCUIT_rules) \\ rw[])
-  THEN1 (
-    Cases \\ rw[Once INE_INSERT]
-    \\ rw[INE_def] \\ metis_tac[]
-  )
+  THEN1 rw[]
 QED
-  
-Definition CIRCUIT_OF_def:
-  CIRCUIT_OF G x l z =
-  (CIRCUIT x l z /\ (!e. e INE PAIRS x l z <=> e INE G))
-End
 
 (*
 Theorem EULER1:
-  !G. FINITE G ==>
+  !G. GRAPH G ==>
   !x y. x IN NODES G /\ z IN NODES G /\
         (if x = z
          then (!v. EVEN (DEG v G))
@@ -274,7 +334,7 @@ Proof
 QED
 *)
 
-val _ = export_theory ()
+export_theory ();
 
 
 
